pulse/share/steel/examples/pulse/by-example/PulseTutorial.SpinLock.fst
@@ -1,0 +1,102 @@
+module PulseTutorial.SpinLock
+open Pulse.Lib.Pervasives
+module Box = Pulse.Lib.Box
+module U32 = FStar.UInt32
+
+let maybe (b:bool) (p:vprop) =
+    if b then p else emp
+
+let lock_inv (r:ref U32.t) (p:vprop) =
+  exists* v. pts_to r v ** maybe (v = 0ul) p
+
+noeq
+type lock (p:vprop) = {
+  r:ref U32.t;
+  i:inv (lock_inv r p);
+}
+
+```pulse
+fn new_lock (p:vprop)
+requires p
+returns l:lock p
+ensures emp
+{
+   let r = Box.alloc 0ul;
+   Box.to_ref_pts_to r;
+   fold (maybe (0ul = 0ul) p);
+   fold (lock_inv (Box.box_to_ref r) p);
+   let i = new_invariant (lock_inv (Box.box_to_ref r) p);
+   let l = { r = Box.box_to_ref r; i };
+   l
+}
+```
+
+
+```pulse
+ghost
+fn elim_cond_true (b:bool) (p q:vprop)
+requires (cond b p q ** pure (b == true))
+ensures p
+{
+  rewrite (cond b p q) as p;
+}  
+```
+
+```pulse
+ghost
+fn elim_cond_false b p q
+requires (cond b p q ** pure (b == false))
+ensures q
+{
+  rewrite (cond b p q) as q;
+}  
+```
+
+```pulse
+fn rec acquire #p (l:lock p)
+requires emp
+ensures p
+{
+  let b = 
+    with_invariants l.i
+    returns b:bool
+    ensures maybe b p {
+        unfold lock_inv;
+        let b = cas l.r 0ul 1ul;
+        if b
+        { 
+          elim_cond_true _ _ _;
+          with _b. rewrite (maybe _b p) as p;
+          fold (maybe false p);
+          rewrite (maybe false p) as (maybe (1ul = 0ul) p);
+          fold (lock_inv l.r p);
+          fold (maybe true p);
+          true
+        }
+        else
+        {
+          elim_cond_false _ _ _;
+          fold (lock_inv l.r p);
+          fold (maybe false p);
+          false
+        }
+  };
+  if b { rewrite (maybe b p) as p; }
+  else { rewrite (maybe b p) as emp; acquire #p l }
+}
+```
+
+```pulse
+fn release #p (l:lock p)
+requires p
+ensures emp
+{
+  with_invariants l.i {
+    unfold lock_inv;
+    write_atomic l.r 0ul;
+    drop_ (maybe _ _); //double release
+    fold (maybe (0ul = 0ul) p);
+    fold (lock_inv l.r p);
+  }
+}
+```
